Common C/Kremlin tests for HMAC

secure_api/hkdf/C.ml
@@ -1,0 +1,75 @@
+open FStar_Buffer
+
+let exit_success = 0
+let exit_failure = 255
+
+let string_of_literal s = s
+let print_string = print_string
+
+let print_bytes b len = Crypto_Symmetric_Bytes.print_buffer b 0 len
+
+let htole16 n = if Sys.big_endian then failwith "Not implemented" else n
+let le16toh n = if Sys.big_endian then n else failwith "Not implemented"
+
+let htole32 n = if Sys.big_endian then failwith "Not implemented" else n
+let le32toh n = if Sys.big_endian then n else failwith "Not implemented"
+
+let htole64 n = if Sys.big_endian then failwith "Not implemented" else n
+let le64toh n = if Sys.big_endian then n else failwith "Not implemented"
+
+let htobe16 n = if Sys.big_endian then failwith "Not implemented" else n
+let be16toh n = if Sys.big_endian then n else failwith "Not implemented"
+
+let htobe32 n = if Sys.big_endian then failwith "Not implemented" else n
+let be32toh n = if Sys.big_endian then n else failwith "Not implemented"
+
+let htobe64 n = if Sys.big_endian then failwith "Not implemented" else n
+let be64toh n = if Sys.big_endian then n else failwith "Not implemented"
+
+let store32_le =
+  let len = FStar_UInt32.uint_to_t (Prims.parse_int "4") in
+  Crypto_Symmetric_Bytes.store_uint32 len
+
+let store32_be =
+  let len = FStar_UInt32.uint_to_t (Prims.parse_int "4") in
+  Crypto_Symmetric_Bytes.store_big32 len
+
+let store64_le =
+  let len = FStar_UInt32.uint_to_t (Prims.parse_int "8") in
+  Crypto_Symmetric_Bytes.store_uint64 len
+
+let store64_be =
+  let len = FStar_UInt32.uint_to_t (Prims.parse_int "8") in
+  Crypto_Symmetric_Bytes.store_big64 len
+
+let store128_le =
+  let len = FStar_UInt32.uint_to_t (Prims.parse_int "16") in
+  Crypto_Symmetric_Bytes.store_uint128 len
+
+let store128_be =
+  let len = FStar_UInt32.uint_to_t (Prims.parse_int "16") in
+  Crypto_Symmetric_Bytes.store_big128 len
+
+let load32_le =
+ let len = FStar_UInt32.uint_to_t (Prims.parse_int "4") in
+ Crypto_Symmetric_Bytes.load_uint32 len
+
+let load32_be =
+ let len = FStar_UInt32.uint_to_t (Prims.parse_int "4") in
+  Crypto_Symmetric_Bytes.load_big32 len
+
+let load64_le =
+ let len = FStar_UInt32.uint_to_t (Prims.parse_int "8") in
+  Crypto_Symmetric_Bytes.load_uint64 len
+
+let load64_be =
+ let len = FStar_UInt32.uint_to_t (Prims.parse_int "8") in
+  Crypto_Symmetric_Bytes.load_big64 len
+
+let load128_le =
+ let len = FStar_UInt32.uint_to_t (Prims.parse_int "16") in
+  Crypto_Symmetric_Bytes.load_uint128 len
+
+let load128_be =
+ let len = FStar_UInt32.uint_to_t (Prims.parse_int "16") in
+  Crypto_Symmetric_Bytes.load_big128 len
